\documentclass{article}
% Comment the following line to NOT allow the usage of umlauts
\usepackage[utf8]{inputenc}

\usepackage{amsfonts, amsthm, amsmath, braket} 
\usepackage{changepage}
\usepackage{tikz}
\usetikzlibrary{angles, quotes, calc, patterns}
\definecolor{cadetgrey}{rgb}{0.57, 0.64, 0.69}
% Uncomment the following line to allow the usage of graphics (.png, .jpg)
%\usepackage{graphicx}


% Start the document
\begin{document}

% Create a new 1st level heading

For orthogonal
\[
c^2 = a^2 + b^2
\]

For any obtuse 

\[
c^2 = a^2 + b^2 + 2ad
\]

dimana $d$ adalah proyeksi $b$ pada $a$.

Komposisi dari Komponen - komponen dengan Titik Aplikasi Bersama.

\begin{tikzpicture}
%the vectors
\draw [->, black] (1.0,0) -- (5.0,0.0);
\draw [black] (3.25, -0.5) node [black]{$v_1$};

\draw [->, black] (1.0,0) -- (3.0,4.0);
\draw (1.5, 2.0) node [black]{$v_2$}; 
\draw [black, <->] (2.7,0) arc (0:44:2.7); 
\draw (2., 1.25) node {$\theta_2$};

%the shadow
\draw [-, black] (5.0, 0,0) -- (7.0,4.0);
\draw [-, black] (3.0,4.0) -- (7.0,4.0);

%the resultant
\draw [->, black] (1.0,0) -- (7.0,4.0);
\draw [black] (3.5, 2.0) node [black]{$r$}; 
\draw [black, <->] (2.0,0) arc (0:35:1);
\draw (1.7, .25) node {$\theta$};

\draw [black] (.75, -.25) node {$O$}; 
\draw [black] (5.25, -.25) node {$A$}; 
\draw [black] (3.15, 4.25) node {$B$}; 
\draw [black] (7.0, 4.25) node {$C$}; 
\end{tikzpicture}

\begin{align*}
OA &= v_1/0 \\
OB &= v_2/\theta_2\\
OC &= r/\theta\\
r^2 &= v_1^2 + v_2^2 + 2v_1v_2\cos\theta\\
\tan\theta &= \frac{v_2\sin\theta_2}{v_1 + v_2\cos\theta_2};
\end{align*}

\begin{tikzpicture}
%common point
\draw [black] (0.875, -0.125) node {$O$};
%the vectors
\draw [->, black] (1.0,0) -- (5.0,2.0);
\draw [black] (5.125, 1.875) node {$A$};
\draw [dotted] (3.5, 0.5) node [black]{($v_1$, $\theta_1$)};
\draw [black, <->] (4.0,0) arc (0:26:3.0); 

\draw [->, black] (1.0,0) -- (2.0,2.0);
\draw [black] (1.825, 2.125) node {$B$};
\draw [dotted] (.75, 1.) node [black]{($v_2$, $\theta_2$)};
\draw [black, <->] (2.0,0) arc (0:63:1.); 

%the shadow
\draw [-, black] (5.0, 2,0) -- (6.0,4.0);
\draw [-, black] (2.0,2.0) -- (6.0,4.0);
%the resultant
\draw [->, black] (1.0,0) -- (6.0,4.0);
\draw [black] (6.125, 4.125) node {$C$};
\draw [dotted] (2.5, 1.35) node [black]{($r$, $\theta$)};
\draw [black, <->] (2.5,0) arc (0:38:1.5); 
\end{tikzpicture}

\begin{align*}
OA &= v_1/\theta_1 \\
OB &= v_2/\theta_2\\
OC &= r/\theta\\
r^2 &= v_1^2 + v_2^2 + 2v_1v_2\cos(\theta2 - \theta_1)\\
\tan\theta &= \frac{v_1\sin\theta_1 + v_2\sin\theta_2}{v_1\cos\theta_1 + v_2\cos\theta_2}\\
r &= \sqrt{v_1^2 + v_2^2 + 2v_1v_2\cos(\theta2 - \theta_1)}\\
\theta &= \tan^{-1}{\frac{v_1\sin\theta_1 + v_2\sin\theta_2}{v_1\cos\theta_1 + v_2\cos\theta_2}}
\end{align*} 


When the components are equal

$r$ is
\begin{align*}
r &= \sqrt{v_1^2 + v_1^2 + 2v_1v_1\cos\theta_2}\\
r &= \sqrt{2v_1^2 + 2v_1^2\cos\theta_2}\\
r &= \sqrt{2v_1^2 (1 + \cos\theta_2)}\\
r &= \sqrt{4v_1^2 \frac{1 + \cos\theta_2}{2}}\\
r &= \sqrt{4v_1^2 \cos^2\frac{\theta_2}{2}}\\
r &= 2v_1\cos\frac{\theta_2}{2}
\end{align*}

$\theta$ is
\begin{align*}
\theta &= \arctan\frac{v_1\sin0 + v_1\sin\theta_2}{v_1\cos0 + v_1\cos\theta_2}\\
\theta &= \arctan\frac{v_1\sin\theta_2}{v_1 + v_1\cos\theta_2}\\ 
\theta &= \arctan\tan\frac{\theta_2}{2}\\
\theta &= \frac{\theta_2}{2}
\end{align*}


\begin{tikzpicture}
%the vectors
\draw [->, black] (1.0,0) -- (5.0,0.0);
\draw [black] (3.25, -0.5) node [black]{$v_1$};

\draw [->, red] (1.0,0) -- (3.0,4.0);
\draw (1.5, 2.0) node [red]{$v_2$}; 
\draw [red, <->] (2.7,0) arc (0:44:2.7); 
\draw (2., 1.25) node [red]{$\theta_2$};

%the shadow
\draw [-, black] (5.0, 0,0) -- (7.0,4.0);
\draw [-, black] (3.0,4.0) -- (7.0,4.0);

%the resultant
\draw [->, black] (1.0,0) -- (7.0,4.0);
\draw [black] (3.5, 2.0) node [black]{$r$}; 
\draw [black, <->] (2.0,0) arc (0:35:1);
\draw (1.7, .25) node {$\theta$};

\draw [black] (.75, -.25) node {$O$}; 
\draw [black] (5.25, -.25) node {$A$}; 
\draw [black] (3.15, 4.25) node {$B$};
\draw [black] (7.0, 4.25) node {$C$}; 
\end{tikzpicture}

Dengan $r$, $v_1$, $\theta$ diketahui, carilah nilai $\theta_2$ dan $v_2$ ($OB$)!

\begin{tikzpicture}
%the vectors
\draw [->, black] (1.0,0) -- (5.0,0.0);
\draw [black] (3.25, -0.5) node [black]{$v_1$};

\draw [->, blue] (1.0,0) -- (-3.0,0.0);
\draw (-1.25, -0.5) node [blue]{$-v_1$};

\draw [->, green] (-3.0,0) -- (3.0,4.0);
\draw [green] (-.5, 2.0) node {$r$}; 

\draw [->, red] (1.0,0) -- (3.0,4.0);
\draw (1.5, 2.0) node [red]{$v_2$}; 
\draw [red, <->] (2.7,0) arc (0:44:2.7); 
\draw (2., 1.25) node [red]{$\theta_2$};

%the shadow
\draw [-, black] (5.0, 0,0) -- (7.0,4.0);
\draw [-, black] (3.0,4.0) -- (7.0,4.0);

%the resultant
\draw [->, black] (1.0,0) -- (7.0,4.0);
\draw [black] (3.5, 2.0) node [black]{$r$}; 
\draw [black, <->] (2.0,0) arc (0:35:1);
\draw (1.7, .25) node {$\theta$};

\draw [black] (.75, -.25) node {$O$}; 
\draw [black] (5.25, -.25) node {$A$}; 
\draw [black] (3.15, 4.25) node {$B$}; 
\draw [black] (7.0, 4.25) node {$C$}; 
\end{tikzpicture}

Garis $OB$ sama dengan diagonal jajaran genjang yang dibentuk oleh
$OC$ dan $OA$ dibalik.

$v_2$ atau $OB$ adalah:

\begin{align*}
v_2 &= \sqrt{(-v_1)^2 + r^2 + 2v_1r\cos(\pi - \theta_2)}\\
v_2 &= \sqrt{v_1^2 + r^2 - 2v_1r\cos\theta_2}\\
\end{align*}

$\theta_2$ is

\begin{align*}
\theta_2 &= \frac{r\sin\theta}{-v_1 + r\cos\theta}
\end{align*}

\begin{tikzpicture}
%common point
\draw [black] (0.875, -0.125) node {$O$};
%the vectors
\draw [dashed, ->, cadetgrey] (1.0,0.0) -- (8.0,0.0);
\draw [dashed, ->, cadetgrey] (1.0,0.0) -- (1.0,5.0);

\draw [thick, ->, black] (1.0,0.0) -- (7.0,3.0);
\draw [black] (7.125, 3.175) node {$i$};
\draw [->, green] (1.0,0) -- (5.0,2.0);
\draw [green] (5.125, 1.875) node {$A$};
\draw (4.2, 0.7) node [blue]{$\theta_1$};
\draw [dotted] (3.2, 0.85) node [green]{$v_1$};
\draw [blue, <->] (4.0,0) arc (0:26:3.0); 

\draw [thick, ->, black] (1.0,0) -- (3.,4.0);
\draw [black] (3.125, 4.125) node {$j$};
\draw [->, green] (1.0,0) -- (2.0,2.0);
\draw [green] (1.825, 2.125) node {$B$};
\draw [dotted] (1.45, 1.4) node [green]{$v_2$};
\draw [dotted] (1.8, 1.) node [cyan]{$\theta_2$};
\draw [cyan, <->] (2.0,0) arc (0:63:1.); 

%the shadow
\draw [-, black] (5.0, 2,0) -- (6.0,4.0);
\draw [-, black] (2.0,2.0) -- (6.0,4.0);
%the resultant
\draw [->, black] (1.0,0) -- (6.0,4.0);
\draw [black] (6.125, 4.125) node {$C$};
\draw [dotted] (3, 1.8) node [black]{$r$};
\draw (2.5, 1.) node [red]{$\theta$};
\draw [red, <->] (2.5,0) arc (0:38:1.5); 
\end{tikzpicture}

 \begin{align*}
v_1 + v_2\cos (\theta_2 - \theta_1) &= r \cos(\theta - \theta_1)\\
v_1 \cos(\theta_2 - \theta_1) + v_2 &= r \cos(\theta_2 - \theta)\\
\end{align*}

so

\begin{align*}
v_1 + v_2\cos (\theta_2 - \theta_1) &= r \cos(\theta - \theta_1)\\
v_1 \cos(\theta_2 - \theta_1)\cos(\theta_2 - \theta_1) + v_2 \cos(\theta_2 - \theta_1) &= r \cos(\theta_2 - \theta) \cos(\theta_2 - \theta_1)\\
v_1(1 - \cos^2(\theta_2 - \theta_1)) &= r(\cos(\theta - \theta_1) - \cos(\theta_2 - \theta)\cos(\theta_2 - \theta_1) )\\
v_1 &= r\frac{(\cos(\theta - \theta_1) - \cos(\theta_2 - \theta)\cos(\theta_2 - \theta_1) )}{(1 - \cos^2(\theta_2 - \theta_1))}\\
\end{align*}

%\begin{tikzpicture} 
%% Draw the first line with absolute coordinates and the 
%% second with relative coordinates to the first line
%\draw (0,0) -- (30:3cm) -- ++(80:3cm); 
%\end{tikzpicture}

example let :

$100/60^\circ, 30^\circ, 60^\circ$

\begin{tikzpicture} 
%\draw (0,0) -- (10:3) -- ++(30:3); 
\draw (0,0) -- (30:5.77) -- ++(90:5.77);
\draw (0,0) -- (60:10);
\draw (0,0) -- (90:5.77) -- ++(30:5.77);
\draw (2.7, 1.2) node [blue] {$v_1$};
\draw (2.7, 4.2) node [black] {$r$};
\draw (-.5, 3.5) node [blue] {$v_2$};
\draw [dashed, cadetgrey, ->](0,0) -- (90:8);
\draw [dashed, cadetgrey, ->](0,0) -- (0:8);
\draw [black, <->] (.5,0) arc (0:90:.5); 
\draw [black] (.20, 1) node {\rotatebox{90}{$90^\circ$}};
\draw [black] (.65, .70) node {\rotatebox{60}{$60^\circ$}};
\draw [black] (1., .25) node {\rotatebox{30}{$30^\circ$}};
\end{tikzpicture}

\begin{align*}
v_1 &= r\frac{\cos(\theta - \theta_1) - \cos(\theta_2 - \theta)\cos(\theta_2 - \theta_1) }{(1 - \cos^2(\theta_2 - \theta_1))}\\
v_1 &= 100\frac{\cos(60^\circ-30^\circ) - \cos(90^\circ - 60^\circ)\cos(90^\circ - 30^\circ)}{1 - \cos^2(90^\circ - 30^\circ)}\\
v_1 &= 100\frac{\cos(30^\circ) - \cos(30^\circ)\cos(60^\circ)}{1 \cos^2(60^\circ)}\\
v_1 &= 100\frac{\cos(30^\circ)(1-cos(60^\circ))}{1-\cos^2(60^\circ)}\\
v_1 &= 100\frac{\cos(30^\circ)(1-\cos(60^\circ))}{(1-\cos(60^\circ))(1+\cos(60^\circ))}\\
v_1 &= 100\frac{\cos(30^\circ)}{1+\cos(60^\circ)}\\
\end{align*}

Komposisi beberapa vektor dengan titik awal bersama. $Resultant$ nya dapat 
diperoleh dengan konstruksi grafix berikut: Ambil vektor dengan sembarang 
urutan, misal $A$, $B$, $C$. Dari titik akhir $A$ gambarkan $\grave{B}$ yang 
sama panjang dan paralel dengan $B$, dan dari titik akhir $\grave{B}$ tarik 
vektor $\grave{C}$ yang sama panjang dan paralel dengan $C$. Vektor yang 
bermula dari $A$ dan berakhir di $\grave{C}$ adalah $Resultant$ dari 
vektor - vektor tersebut. $Resultant$ yang didapat sama tanpa memperhatikan 
urutan vektor, dan karena urutannya tidak menentukan area yang diliputi.

Hasilnya dapat di peroleh secara analitis sebagai berikut.
Misalkan 
\[
f_1/\underline{\theta_1} + f_2/\underline{\theta_2} +  ... + f_n/\underline{\theta_n}.
\]
sekarang
\[
f_1/\underline{\theta_1} = f_1\cos\theta_1/\underline{0} + f_1\sin\theta_1/\underline{\frac{\pi}{2}} 
\]
juga
\[
f_2/\underline{\theta_2} = f_2\cos\theta_2/\underline{0} + f_2\sin\theta_2/\underline{\frac{\pi}{2}} 
\]
dan
\[
f_n/\underline{\theta_n} = f_n\cos\theta_n/\underline{0} + f_n\sin\theta_n/\underline{\frac{\pi}{2}} 
\]
dengan demikian
\begin{align*}
\sum\Bigl\lbrace f/\theta \Bigr\rbrace &= \Bigl\lbrace \sum{f \cos\theta}\Bigr\rbrace/0 + \Bigl\lbrace\sum{f \sin\theta}\Bigr\rbrace/\frac{\pi}{2}\\
&=\sqrt{(\sum{f \cos\theta})^2 + (\sum{f \sin \theta})^2}/\tan^{-1}\frac{\sum f \sin \theta}{\sum f \cos \theta}
\end{align*}

Quaternion
\begin{align*}
(\alpha_1, 0) (a_1, a_2) &= (\alpha_1 a_1, \alpha_1 a_2)\\
(\alpha_1, \alpha_2) (a_1, 0) &= (\alpha_1 a_1, \alpha_2 a_1)\\
(0, \alpha_2)(0, a_2) &= (-1 \alpha_2 a_2, 0 \alpha_2 a_2)\\
(\alpha_1, \alpha_2) &= (\alpha_1, 0) + (0, \alpha_2)\\
(\alpha_1, \alpha_2) (a_1, a_2) &= (\alpha_1, 0)(a_1, a_2) + (0, \alpha_2)(a_1, a_2)\\
(\alpha_1, \alpha_2) (a_1, a_2) &= (\alpha_1 a_1, \alpha_1 a_2) + (0, \alpha_2)(a_1, a_2)\\
(\alpha_1, \alpha_2) (a_1, a_2) &= (\alpha_1 a_1, \alpha_1 a_2) + (0, \alpha_2)(0, a_2) + (0, \alpha_2)(a_1, 0)\\
(\alpha_1, \alpha_2) (a_1, a_2) &= (\alpha_1 a_1, \alpha_1 a_2) + (-\alpha_2 a_2, 0) + (0, \alpha_2)(a_1, 0)\\
(\alpha_1, \alpha_2) (a_1, a_2) &= (\alpha_1 a_1, \alpha_1 a_2) + (-\alpha_2 a_2, 0) + (a_1 0, a_1 \alpha_2)\\
(\alpha_1, \alpha_2) (a_1, a_2) &= (\alpha_1 a_1 -\alpha_2 a_2 , \alpha_1 a_2 + \alpha_2 a_1)
\end{align*}

Quaternion15
\begin{align*}
(0, 1)(a, b) &= (0, 1)(a, 0) + (0, 1)(0, b)\\
(0, 1)(a, b) &= (0, a) + (-b, 0)\\
(0, 1)(a, b) &= (-b, a)
\end{align*}

Examples To Try
\begin{align*}
(4 + 3i)\cdot i &=  4i -3\\
(4 + 3i)\cdot 2i &=  8i -6\\
(4 + 3i)\cdot (4 + 3i) &=  16 + 12i + 12i + 9i^2\\
&= 16 + 24i -9\\
&= 7 + 24i\\
(2 + i)(1 + 2i) &= 2 + 5i -2\\
&= 5i
\end{align*} 


\textbf{del Ferro - Cardan - Bombelli}

Solutions to quadration equation

\begin{align*}
ax^2 + bx + c &= 0\\
ax^2 &= -bx - c\\
ax^2 &= -bx - c\\
\frac{ax^2}{b} &= -\frac{bx}{b} - \frac{c}{b}\\ 
\frac{a}{b}x\times x + x&= -\frac{c}{b}\\
(\frac{a}{b}x + 1)\times x &= -\frac{c}{b}
\end{align*}

\textbf{Solving quadration equation}
\begin{enumerate}

\item \textit{Factoring by Inspection}

It is almost possible to factorize quadratic equation $ax^2 + bx + c$ into
$(px + q)(rx + s)$. By dividing the first equation with $a$ second equation
can be expressed as $(x + q)(x + s)$. $q$ and $s$ in turns should be equals
to $b$ if added up and and the product equals to $c$. In case either $b$ or $c$
is $0$ factoring by inspection will fail.




\item \textit{Completing the square}

The process of completing the square makes use of algebraic identity

\[
x^2 + 2hx + h^2 = (x + h)^2
\]

for example 
\begin{align*}
(x + 3) ^2 &= x^2 + 6x + 9     &(p = 3)\\
(x - 5) ^2 &= x^2 - 10x + 25   &(p = -5)
\end{align*}

The steps of completing the square

\begin{enumerate}
\item Divide each side by $a$, the coefficient of square term
\item Subtract the constant term $c\div a$ from both sides
\item Add the square of one-half $b\div a$, the coefficient of x, to both sides.
This "completes the square", converting the left side into a perfect square
\item Write the left side as a square and simplify the right side if necessary.
\item Produce two linear equations by equating the square root of the left side
with positive and negative square roots of the right side.
\item Solve each of the two linear equations.
\end{enumerate}

example
\[
x^2 + 10x + 28 = 0
\]

we know that
\[
(x + 5)^2 = x^2 + 10x + 25
\]

\begin{align*}
x^2 + 10x + 28 &= (x + 5)^2 + 3\\
(x + 5)^2 + 3&= 0\\
(x + 5)^2 &= -3\\ 
(x + 5) &= \pm\sqrt{-3}\\
x  &= -5 \pm\sqrt{-3}
\end{align*}

Another example

\begin{align*}
x^2 + 6x + 5 &= 0\\
(x + 3)^2 - 4 &= 0\\
(x + 3)^2 &= 4\\
x + 3 &= \pm \sqrt{4}\\
x  &= -3 \pm 2\\
\end{align*}

try to summarize with picture
\begin{figure}
\begin{adjustwidth*}{2em}{}
\begin{tikzpicture}
\draw (0, 1) [anchor=east] node {x} ;
\draw (0, 0) [gray, fill=gray] rectangle +(2, 2) (4, 0) rectangle +(.8, 2) ;
\draw (1, 2) [black, anchor=south] node {x};
\draw (3, 1) [black] node{+};
\draw (6, 1) [black] node{+};
\draw (4.4, 0)[black, -, dashed] -- (4.4, 2);
\draw (4, 0) [anchor = north east] node {$\frac{b}{2a}x$};
\draw (4.8, 0) [anchor = north west] node {$\frac{b}{2a}x$};
\draw (7, 1) node {$\frac{c}{a}$};
\draw (8, 1) [black] node{=};
\draw (9, 1) [black] node{0};
\end{tikzpicture}

\begin{tikzpicture}
\draw (0, 1) [anchor=east] node {x} ;
\draw (0, 0) [gray, fill=gray] rectangle +(2, 2) (4, 0) rectangle +(.8, 2) ;
\draw (1, 2) [black, anchor=south] node {x};
\draw (3, 1) [black] node{+};
%\draw (6, 1) [black] node{+};
\draw (4.4, 0)[black, -, dashed] -- (4.4, 2);
\draw (4, 0) [anchor = north east] node {$\frac{b}{2a}x$};
\draw (4.8, 0) [anchor = north west] node {$\frac{b}{2a}x$};
\draw (7, 1) node {$-\frac{c}{a}$};
\draw (6, 1) [black] node{=};
%\draw (9, 1) [black] node{0};
\end{tikzpicture}

\begin{tikzpicture}
\draw (0, 1) [anchor=east] node {x} ;
\draw (0, 0) [gray, fill=gray] rectangle +(2, 2) (0, 2) rectangle +(2, .4) (2, 0) rectangle +(.4, 2);
\draw (1, 0) [black, anchor=north] node {x};
\draw (2, 2)[black, -, dashed] -- (0, 2) (0, 2.4)node [anchor=south west] {$\frac{b}{2a}x$};
\draw (2, 2)[black, -, dashed] -- (2, 0) node [anchor=north west] {$\frac{b}{2a}x$};
\draw (2, 2)[red, -,  fill=blue] rectangle +(.4, .4);
\draw (2.2, 2.4) node [anchor = south]{$\frac{b}{2a}$};
\draw (2.4, 2.2) node [anchor = west]{$\frac{b}{2a}$};
\draw (3, 1) [black] node{=};
\draw (4, 1) [black] node {$-\frac{c}{a} + \frac{b^2}{4a^2}$};
\end{tikzpicture}


\begin{tikzpicture}
\draw (0, 1) [anchor=east] node {x};
\draw (0, 0) [gray, fill=gray] rectangle +(2, 2) (0, 2) rectangle +(2, .4) (2, 0) rectangle +(.4, 2);
\draw (1, 0) [black, anchor=north] node {x};
\draw (2, 2)[black, -, dashed] -- (0, 2) (0, 2.4)node [anchor=south west] {$\frac{b}{2a}x$};
\draw (2, 2)[black, -, dashed] -- (2, 0) node [anchor=north west] {$\frac{b}{2a}x$};
\draw (2, 2)[red, -,  fill=blue] rectangle +(.4, .4);
\draw (2.2, 2.4) node [anchor = south]{$\frac{b}{2a}$};
\draw (2.4, 2.2) node [anchor = west]{$\frac{b}{2a}$};
\draw (3, 1) [black] node{=};
\draw (4, 1) [black] node {$-\frac{4ac}{4a^2} + \frac{b^2}{4a^2}$};
\end{tikzpicture}

\begin{tikzpicture}
\draw (0, 1) [anchor=east] node {x} ;
\draw (0, 0) [gray, fill=gray] rectangle +(2, 2) (0, 2) rectangle +(2, .4) (2, 0) rectangle +(.4, 2);
\draw (1, 0) [black, anchor=north] node {x};
\draw (2, 2)[black, -, dashed] -- (0, 2) (0, 2.4)node [anchor=south west] {$\frac{b}{2a}x$};
\draw (2, 2)[black, -, dashed] -- (2, 0) node [anchor=north west] {$\frac{b}{2a}x$};
\draw (2, 2)[red, -,  fill=blue] rectangle +(.4, .4);
\draw (2.2, 2.4) node [anchor = south]{$\frac{b}{2a}$};
\draw (2.4, 2.2) node [anchor = west]{$\frac{b}{2a}$};
\draw (3, 1) [black] node{=};
\draw (4, 1) [black] node {$\frac{b^2 - 4ac}{4a^2}$};
\end{tikzpicture}
\end{adjustwidth*}
\end{figure}

which can be equal for for equation
\[ax^2 + bx + c = 0\] 
\begin{align*}
 x^2 + \frac{b}{a} + \frac{c}{a} &= 0\\
 x^2 + \frac{b}{a} &= - \frac{c}{a}\\
 x^2 + \frac{b}{a} + \frac{b^2}{4a^2} &= - \frac{c}{a} + \frac{b^2}{4a^2}\\
 (x + \frac{b}{2a})^2 &= - \frac{c}{a} + (\frac{b}{2a})^2\\
 (x + \frac{b}{2a})^2 &= - \frac{c}{a} + (\frac{b2}{4a^2})\\
 (x + \frac{b}{2a})^2 &= - \frac{4ac}{4a^2} + (\frac{b2}{4a^2})\\
 (x + \frac{b}{2a})^2 &= \frac{b2 - 4ac}{4a^2}\\
  x + \frac{b}{2a} &= \sqrt{\frac{b2 - 4ac}{4a^2}}\\
  x &= - \frac{b}{2a} \pm \sqrt{\frac{b2 - 4ac}{4a^2}}\\
  x &= - \frac{b \pm \sqrt{b2 - 4ac}}{2a}
\end{align*}
\end{enumerate} 
\end{document}
